@prefix : <http://purl.org/query/voidext#> .
@prefix owl: <http://www.w3.org/2002/07/owl#> .
@prefix rdf: <http://www.w3.org/1999/02/22-rdf-syntax-ns#> .
@prefix xml: <http://www.w3.org/XML/1998/namespace> .
@prefix xsd: <http://www.w3.org/2001/XMLSchema#> .
@prefix rdfs: <http://www.w3.org/2000/01/rdf-schema#> .
@base <http://purl.org/query/voidext> .

<http://purl.org/query/voidext> rdf:type owl:Ontology ;
                                 <http://purl.org/dc/terms/created> "2019-01-30"^^xsd:date ;
                                 <http://purl.org/dc/terms/creator> <http://purl.org/query/tarcisiomf> ;
                                 <http://purl.org/dc/terms/description> "The Extension of the Vocabulary of Interlinked Datasets (VoID) RDF Schema to include the concept of virtual links. This extension enhances interoperability among heterogeneous and distributed RDF data sets by bridging them through explicitly defined virtual links."^^xsd:string ;
                                 <http://purl.org/dc/terms/isVersionOf> <http://rdfs.org/ns/void.ttl> ;
                                 <http://purl.org/dc/terms/license> <https://creativecommons.org/licenses/by/3.0/> ;
                                 <http://purl.org/dc/terms/modified> "2019-03-30"^^xsd:date ;
                                 <http://purl.org/dc/terms/publisher> ""^^xsd:string ;
                                 <http://purl.org/dc/terms/status> <http://purl.org/adms/status/UnderDevelopment> ;
                                 <http://purl.org/dc/terms/title> "Extended Vocabulary of Interlinked Datasets (VoIDext)"^^xsd:string ;
                                 <http://purl.org/dc/terms/type> <http://purl.org/adms/assettype/Ontology> ;
                                 <http://purl.org/vocab/vann/preferredNamespacePrefix> "voidext"^^xsd:string ;
                                 <http://purl.org/vocab/vann/preferredNamespaceUri> "http://purl.org/query/voidext#"^^xsd:string ;
                                 <http://xmlns.com/foaf/0.1/homepage> <http://purl.org/query/voidext> .

#################################################################
#    Annotation properties
#################################################################

###  http://purl.org/dc/terms/contributor
<http://purl.org/dc/terms/contributor> rdf:type owl:AnnotationProperty .


###  http://purl.org/dc/terms/created
<http://purl.org/dc/terms/created> rdf:type owl:AnnotationProperty .


###  http://purl.org/dc/terms/creator
<http://purl.org/dc/terms/creator> rdf:type owl:AnnotationProperty .


###  http://purl.org/dc/terms/description
<http://purl.org/dc/terms/description> rdf:type owl:AnnotationProperty .


###  http://purl.org/dc/terms/issued
<http://purl.org/dc/terms/issued> rdf:type owl:AnnotationProperty .


###  http://purl.org/dc/terms/label
<http://purl.org/dc/terms/label> rdf:type owl:AnnotationProperty .


###  http://purl.org/dc/terms/modified
<http://purl.org/dc/terms/modified> rdf:type owl:AnnotationProperty .


###  http://purl.org/dc/terms/provenance
<http://purl.org/dc/terms/provenance> rdf:type owl:AnnotationProperty .


###  http://rdfs.org/ns/void#rootResource
<http://rdfs.org/ns/void#rootResource> <http://purl.org/dc/terms/creator> <http://vocab.deri.ie/void#cygri> ,
                                                                          <http://vocab.deri.ie/void#junzha> ,
                                                                          <http://vocab.deri.ie/void#keiale> ,
                                                                          <http://vocab.deri.ie/void#Michael%20Hausenblas> ;
                                       rdfs:comment "A top concept or entry point for a void:Dataset that is structured in a tree-like fashion. All resources in a dataset can be reached by following links from its root resources in a small number of steps."^^xsd:string ;
                                       rdfs:isDefinedBy <http://vocab.deri.ie/void> ;
                                       rdfs:label "root resource"^^xsd:string ;
                                       rdf:type owl:AnnotationProperty ;
                                       rdfs:domain <http://rdfs.org/ns/void#Dataset> .


###  http://rdfs.org/ns/void#sparqlEndpoint
<http://rdfs.org/ns/void#sparqlEndpoint> <http://purl.org/dc/terms/creator> <http://vocab.deri.ie/void#cygri> ,
                                                                            <http://vocab.deri.ie/void#junzha> ,
                                                                            <http://vocab.deri.ie/void#keiale> ,
                                                                            <http://vocab.deri.ie/void#Michael%20Hausenblas> ;
                                         rdfs:isDefinedBy <http://vocab.deri.ie/void> ;
                                         rdfs:label "has a SPARQL endpoint at"^^xsd:string ;
                                         rdf:type owl:AnnotationProperty ;
                                         rdfs:domain <http://rdfs.org/ns/void#Dataset> .


###  http://rdfs.org/ns/void#uriLookupEndpoint
<http://rdfs.org/ns/void#uriLookupEndpoint> <http://purl.org/dc/terms/creator> <http://vocab.deri.ie/void#cygri> ,
                                                                               <http://vocab.deri.ie/void#junzha> ,
                                                                               <http://vocab.deri.ie/void#keiale> ,
                                                                               <http://vocab.deri.ie/void#Michael%20Hausenblas> ;
                                            rdfs:comment "Defines a simple URI look-up protocol for accessing a dataset."^^xsd:string ;
                                            rdfs:isDefinedBy <http://vocab.deri.ie/void> ;
                                            rdfs:label "has an URI look-up endpoint at"^^xsd:string ;
                                            rdf:type owl:AnnotationProperty ;
                                            rdfs:domain <http://rdfs.org/ns/void#Dataset> .


###  http://rdfs.org/ns/void#uriRegexPattern
<http://rdfs.org/ns/void#uriRegexPattern> <http://purl.org/dc/terms/creator> <http://vocab.deri.ie/void#cygri> ,
                                                                             <http://vocab.deri.ie/void#junzha> ,
                                                                             <http://vocab.deri.ie/void#keiale> ,
                                                                             <http://vocab.deri.ie/void#Michael%20Hausenblas> ;
                                          rdfs:comment "Defines a regular expression pattern matching URIs in the dataset."^^xsd:string ;
                                          rdfs:isDefinedBy <http://vocab.deri.ie/void> ;
                                          rdfs:label "has URI regular expression pattern"^^xsd:string ;
                                          rdf:type owl:AnnotationProperty ;
                                          rdfs:domain <http://rdfs.org/ns/void#Dataset> .


###  http://rdfs.org/ns/void#vocabulary
<http://rdfs.org/ns/void#vocabulary> <http://purl.org/dc/terms/creator> <http://vocab.deri.ie/void#cygri> ,
                                                                        <http://vocab.deri.ie/void#junzha> ,
                                                                        <http://vocab.deri.ie/void#keiale> ,
                                                                        <http://vocab.deri.ie/void#Michael%20Hausenblas> ;
                                     rdfs:comment "A vocabulary that is used in the dataset."^^xsd:string ;
                                     rdfs:isDefinedBy <http://vocab.deri.ie/void> ;
                                     rdfs:label "vocabulary"^^xsd:string ;
                                     rdf:type owl:AnnotationProperty ;
                                     rdfs:domain <http://rdfs.org/ns/void#Dataset> .


###  http://xmlns.com/foaf/0.1/homepage
<http://xmlns.com/foaf/0.1/homepage> rdf:type owl:AnnotationProperty .


###  http://xmlns.com/foaf/0.1/mbox
<http://xmlns.com/foaf/0.1/mbox> rdf:type owl:AnnotationProperty .


###  http://xmlns.com/foaf/0.1/member
<http://xmlns.com/foaf/0.1/member> rdf:type owl:AnnotationProperty .


###  http://xmlns.com/foaf/0.1/name
<http://xmlns.com/foaf/0.1/name> rdf:type owl:AnnotationProperty .


#################################################################
#    Datatypes
#################################################################

###  http://www.w3.org/2001/XMLSchema#date
xsd:date rdf:type rdfs:Datatype .


#################################################################
#    Object Properties
#################################################################

###  http://purl.org/query/voidext#intersectAt
:intersectAt rdf:type owl:ObjectProperty ;
             rdfs:domain :ComplexLinkSet ;
             rdfs:range :SimpleLinkSet ;
             rdfs:comment "This property is used to assign exactly either two shared instance sets (voidext:SharedInstanceSet) or two link sets (void:Linkset) to compose a complex link set (voidext:ComplexLinkSet). For each void:Linkset, either the subject or the object node of its link predicate intersects an RDF node of the link predicate from the other link set. In other words, the subject xor the object of a link predicate matches the subject xor the object of the other link predicate, where xor is the exclusive or. These link predicates must be from different datasets."@en ;
             rdfs:label "intersects at"@en .


###  http://purl.org/query/voidext#intersectionType
:intersectionType rdf:type owl:ObjectProperty ;
                  rdfs:domain :ComplexLinkSet ;
                  rdfs:range :LinkSetIntersection ;
                  rdfs:comment "This property assigns the intersection type of two RDF triples in different datasets (void:Dataset). In other words, if the intersection occurs at the subject xor the object node of a link predicate."@en ;
                  rdfs:label "intersection type"@en .


###  http://purl.org/query/voidext#linkPredicateDomain
:linkPredicateDomain rdf:type owl:ObjectProperty ;
                     rdfs:domain <http://rdfs.org/ns/void#Linkset> ;
                     rdfs:range rdfs:Class ;
                     rdfs:comment "The link predicate's subject type (i.e. class), if any. Moreover, in the case of a void:Linkset that is not part of a complex virtual link (voidext:ComplexLinkset), if the two datasets are linked through the link predicate's subject then the link predicate range must be specified. Indeed, this subject matches a second resource in another dataset. Therefore, the type of this second resource is asserted as the link predicate range."@en ;
                     rdfs:label "link predicate domain"@en .


###  http://purl.org/query/voidext#linkPredicateRange
:linkPredicateRange rdf:type owl:ObjectProperty ;
                    rdfs:domain <http://rdfs.org/ns/void#Linkset> ;
                    rdfs:range rdfs:Class ;
                    rdfs:comment "The link predicate's object type (i.e. class), if any. Moreover, in the case of a void:Linkset that is not part of a complex virtual link, if the two datasets are linked through the link predicate's object then the link predicate range must be specified. Indeed, this object matches a second resource in another dataset. Therefore, the type of this second resource is asserted as the link predicate range."@en ;
                    rdfs:label "link predicate range"@en .


###  http://purl.org/query/voidext#recommendedMapping
:recommendedMapping rdf:type owl:ObjectProperty ,
                             owl:FunctionalProperty ;
                    rdfs:domain :ComplexLinkSet ;
                    rdfs:range :SimpleLinkSet ;
                    rdfs:comment "If more than one mapping is defined in the different void:Linkset(s) that are part of a voidext:ComplexLinkSet, one of the resource mappings may be recommended by asserting this property. The recommended mapping is the one stated to the void:Linkset assigned as the value of this property. If no mapping is explicitly recommended, solely one of them must arbitrarily be applied to establish a virtual link. At most one mapping function can be defined per voidext:SimpleLinkSet."@en ;
                    rdfs:label "recommended mapping from"@en .


###  http://purl.org/query/voidext#sharedInstanceType
:sharedInstanceType rdf:type owl:ObjectProperty ;
                    rdfs:domain :SharedInstanceSet ;
                    rdfs:range rdfs:Class ;
                    rdfs:comment "This property assings the type (i.e. class) of the shared instances from a given void:Dataset. Shared instances implies equivalent or similar instance IRIs that belong to different datasets."@en ;
                    rdfs:label "shared instance type"@en .


###  http://rdfs.org/ns/void#class
<http://rdfs.org/ns/void#class> rdf:type owl:ObjectProperty ,
                                         owl:FunctionalProperty ;
                                rdfs:domain <http://rdfs.org/ns/void#Dataset> ;
                                rdfs:range rdfs:Class ;
                                <http://purl.org/dc/terms/creator> <http://vocab.deri.ie/void#cygri> ,
                                                                   <http://vocab.deri.ie/void#junzha> ,
                                                                   <http://vocab.deri.ie/void#keiale> ,
                                                                   <http://vocab.deri.ie/void#Michael%20Hausenblas> ;
                                rdfs:comment "The rdfs:Class that is the rdf:type of all entities in a class-based partition."^^xsd:string ;
                                rdfs:isDefinedBy <http://vocab.deri.ie/void> ;
                                rdfs:label "class"^^xsd:string .


###  http://rdfs.org/ns/void#classPartition
<http://rdfs.org/ns/void#classPartition> rdf:type owl:ObjectProperty ;
                                         rdfs:subPropertyOf <http://rdfs.org/ns/void#subset> ;
                                         rdfs:domain <http://rdfs.org/ns/void#Dataset> ;
                                         rdfs:range <http://rdfs.org/ns/void#Dataset> ;
                                         <http://purl.org/dc/terms/creator> <http://vocab.deri.ie/void#cygri> ,
                                                                            <http://vocab.deri.ie/void#junzha> ,
                                                                            <http://vocab.deri.ie/void#keiale> ,
                                                                            <http://vocab.deri.ie/void#Michael%20Hausenblas> ;
                                         rdfs:comment "A subset of a void:Dataset that contains only the entities of a certain rdfs:Class."^^xsd:string ;
                                         rdfs:isDefinedBy <http://vocab.deri.ie/void> ;
                                         rdfs:label "class partition"^^xsd:string .


###  http://rdfs.org/ns/void#dataDump
<http://rdfs.org/ns/void#dataDump> rdf:type owl:ObjectProperty ;
                                   rdfs:domain <http://rdfs.org/ns/void#Dataset> ;
                                   rdfs:range rdfs:Resource ;
                                   <http://purl.org/dc/terms/creator> <http://vocab.deri.ie/void#cygri> ,
                                                                      <http://vocab.deri.ie/void#junzha> ,
                                                                      <http://vocab.deri.ie/void#keiale> ,
                                                                      <http://vocab.deri.ie/void#Michael%20Hausenblas> ;
                                   rdfs:comment "An RDF dump, partial or complete, of a void:Dataset."^^xsd:string ;
                                   rdfs:isDefinedBy <http://vocab.deri.ie/void> ;
                                   rdfs:label "Data Dump"^^xsd:string .


###  http://rdfs.org/ns/void#exampleResource
<http://rdfs.org/ns/void#exampleResource> rdf:type owl:ObjectProperty ;
                                          rdfs:domain <http://rdfs.org/ns/void#Dataset> ;
                                          rdfs:range rdfs:Resource ;
                                          <http://purl.org/dc/terms/creator> <http://vocab.deri.ie/void#cygri> ,
                                                                             <http://vocab.deri.ie/void#junzha> ,
                                                                             <http://vocab.deri.ie/void#keiale> ,
                                                                             <http://vocab.deri.ie/void#Michael%20Hausenblas> ;
                                          rdfs:isDefinedBy <http://vocab.deri.ie/void> ;
                                          rdfs:label "example resource of dataset"^^xsd:string .


###  http://rdfs.org/ns/void#feature
<http://rdfs.org/ns/void#feature> rdf:type owl:ObjectProperty ;
                                  rdfs:domain <http://rdfs.org/ns/void#Dataset> ;
                                  rdfs:range <http://rdfs.org/ns/void#TechnicalFeature> ;
                                  <http://purl.org/dc/terms/creator> <http://vocab.deri.ie/void#cygri> ,
                                                                     <http://vocab.deri.ie/void#junzha> ,
                                                                     <http://vocab.deri.ie/void#keiale> ,
                                                                     <http://vocab.deri.ie/void#Michael%20Hausenblas> ;
                                  rdfs:isDefinedBy <http://vocab.deri.ie/void> ;
                                  rdfs:label "feature"^^xsd:string .


###  http://rdfs.org/ns/void#inDataset
<http://rdfs.org/ns/void#inDataset> rdf:type owl:ObjectProperty ;
                                    rdfs:domain <http://xmlns.com/foaf/0.1/Document> ;
                                    rdfs:range <http://rdfs.org/ns/void#Dataset> ;
                                    <http://purl.org/dc/terms/creator> <http://vocab.deri.ie/void#cygri> ,
                                                                       <http://vocab.deri.ie/void#junzha> ,
                                                                       <http://vocab.deri.ie/void#keiale> ,
                                                                       <http://vocab.deri.ie/void#Michael%20Hausenblas> ;
                                    rdfs:comment "Points to the void:Dataset that a document is a part of."^^xsd:string ;
                                    rdfs:isDefinedBy <http://vocab.deri.ie/void> ;
                                    rdfs:label "in dataset"^^xsd:string .


###  http://rdfs.org/ns/void#linkPredicate
<http://rdfs.org/ns/void#linkPredicate> rdf:type owl:ObjectProperty ;
                                        rdfs:domain <http://rdfs.org/ns/void#Linkset> ;
                                        rdfs:range rdf:Property ;
                                        <http://purl.org/dc/terms/creator> <http://vocab.deri.ie/void#cygri> ,
                                                                           <http://vocab.deri.ie/void#junzha> ,
                                                                           <http://vocab.deri.ie/void#keiale> ,
                                                                           <http://vocab.deri.ie/void#Michael%20Hausenblas> ;
                                        rdfs:comment "It specifies the RDF predicate in a given dataset that relates to another dataset. In other words, the link predicate is the RDF property in the predicate position of an RDF triple that links two datasets."^^xsd:string ;
                                        rdfs:isDefinedBy <http://vocab.deri.ie/void> ;
                                        rdfs:label "a link predicate"^^xsd:string .


###  http://rdfs.org/ns/void#objectsTarget
<http://rdfs.org/ns/void#objectsTarget> rdf:type owl:ObjectProperty ;
                                        rdfs:subPropertyOf <http://rdfs.org/ns/void#target> ;
                                        rdf:type owl:FunctionalProperty ;
                                        rdfs:domain :VirtualLink ;
                                        rdfs:range <http://rdfs.org/ns/void#Dataset> ;
                                        <http://purl.org/dc/terms/contributor> <http://purl.org/query/tarcisiomf> ;
                                        <http://purl.org/dc/terms/created> "2010-01-26"^^xsd:date ;
                                        <http://purl.org/dc/terms/creator> <http://vocab.deri.ie/void#cygri> ,
                                                                           <http://vocab.deri.ie/void#junzha> ,
                                                                           <http://vocab.deri.ie/void#keiale> ,
                                                                           <http://vocab.deri.ie/void#Michael%20Hausenblas> ;
                                        <http://purl.org/dc/terms/modified> "2019-01-30"^^xsd:date ;
                                        <http://purl.org/dc/terms/provenance> :MODIFIED_TARGET ;
                                        rdfs:comment "The dataset describing the objects of the triples contained in the virtual link."^^xsd:string ;
                                        rdfs:label "Objects Target"^^xsd:string .


###  http://rdfs.org/ns/void#openSearchDescription
<http://rdfs.org/ns/void#openSearchDescription> rdf:type owl:ObjectProperty ;
                                                rdfs:domain <http://rdfs.org/ns/void#Dataset> ;
                                                rdfs:range <http://xmlns.com/foaf/0.1/Document> ;
                                                <http://purl.org/dc/terms/creator> <http://vocab.deri.ie/void#cygri> ,
                                                                                   <http://vocab.deri.ie/void#junzha> ,
                                                                                   <http://vocab.deri.ie/void#keiale> ,
                                                                                   <http://vocab.deri.ie/void#Michael%20Hausenblas> ;
                                                rdfs:comment "An OpenSearch description document for a free-text search service over a void:Dataset."^^xsd:string ;
                                                rdfs:isDefinedBy <http://vocab.deri.ie/void> ;
                                                rdfs:label "open search description"^^xsd:string .


###  http://rdfs.org/ns/void#property
<http://rdfs.org/ns/void#property> rdf:type owl:ObjectProperty ,
                                            owl:FunctionalProperty ;
                                   rdfs:domain <http://rdfs.org/ns/void#Dataset> ;
                                   rdfs:range rdf:Property ;
                                   <http://purl.org/dc/terms/creator> <http://vocab.deri.ie/void#cygri> ,
                                                                      <http://vocab.deri.ie/void#junzha> ,
                                                                      <http://vocab.deri.ie/void#keiale> ,
                                                                      <http://vocab.deri.ie/void#Michael%20Hausenblas> ;
                                   rdfs:comment "The rdf:Property that is the predicate of all triples in a property-based partition."^^xsd:string ;
                                   rdfs:isDefinedBy <http://vocab.deri.ie/void> ;
                                   rdfs:label "property"^^xsd:string .


###  http://rdfs.org/ns/void#propertyPartition
<http://rdfs.org/ns/void#propertyPartition> rdf:type owl:ObjectProperty ;
                                            rdfs:subPropertyOf <http://rdfs.org/ns/void#subset> ;
                                            rdfs:domain <http://rdfs.org/ns/void#Dataset> ;
                                            rdfs:range <http://rdfs.org/ns/void#Dataset> ;
                                            <http://purl.org/dc/terms/creator> <http://vocab.deri.ie/void#cygri> ,
                                                                               <http://vocab.deri.ie/void#junzha> ,
                                                                               <http://vocab.deri.ie/void#keiale> ,
                                                                               <http://vocab.deri.ie/void#Michael%20Hausenblas> ;
                                            rdfs:comment "A subset of a void:Dataset that contains only the triples of a certain rdf:Property."^^xsd:string ;
                                            rdfs:isDefinedBy <http://vocab.deri.ie/void> ;
                                            rdfs:label "property partition"^^xsd:string .


###  http://rdfs.org/ns/void#subjectsTarget
<http://rdfs.org/ns/void#subjectsTarget> rdf:type owl:ObjectProperty ;
                                         rdfs:subPropertyOf <http://rdfs.org/ns/void#target> ;
                                         rdf:type owl:FunctionalProperty ;
                                         rdfs:domain :VirtualLink ;
                                         rdfs:range <http://rdfs.org/ns/void#Dataset> ;
                                         <http://purl.org/dc/terms/contributor> <http://purl.org/query/tarcisiomf> ;
                                         <http://purl.org/dc/terms/created> "2010-01-26"^^xsd:date ;
                                         <http://purl.org/dc/terms/creator> <http://vocab.deri.ie/void#cygri> ,
                                                                            <http://vocab.deri.ie/void#junzha> ,
                                                                            <http://vocab.deri.ie/void#keiale> ,
                                                                            <http://vocab.deri.ie/void#Michael%20Hausenblas> ;
                                         <http://purl.org/dc/terms/modified> "2019-01-30"^^xsd:date ;
                                         <http://purl.org/dc/terms/provenance> :MODIFIED_TARGET ;
                                         rdfs:comment "The dataset describing the subjects of triples contained in the virtual link."^^xsd:string ;
                                         rdfs:label "Subjects Target"^^xsd:string .


###  http://rdfs.org/ns/void#subset
<http://rdfs.org/ns/void#subset> rdf:type owl:ObjectProperty ;
                                 rdfs:domain <http://rdfs.org/ns/void#Dataset> ;
                                 rdfs:range <http://rdfs.org/ns/void#Dataset> ;
                                 <http://purl.org/dc/terms/creator> <http://vocab.deri.ie/void#cygri> ,
                                                                    <http://vocab.deri.ie/void#junzha> ,
                                                                    <http://vocab.deri.ie/void#keiale> ,
                                                                    <http://vocab.deri.ie/void#Michael%20Hausenblas> ;
                                 rdfs:isDefinedBy <http://vocab.deri.ie/void> ;
                                 rdfs:label "has subset"^^xsd:string .


###  http://rdfs.org/ns/void#target
<http://rdfs.org/ns/void#target> rdf:type owl:ObjectProperty ;
                                 rdfs:domain :VirtualLink ;
                                 rdfs:range <http://rdfs.org/ns/void#Dataset> ;
                                 <http://purl.org/dc/terms/contributor> <http://purl.org/query/tarcisiomf> ;
                                 <http://purl.org/dc/terms/created> "2010-01-26"^^xsd:date ;
                                 <http://purl.org/dc/terms/creator> <http://vocab.deri.ie/void#cygri> ,
                                                                    <http://vocab.deri.ie/void#junzha> ,
                                                                    <http://vocab.deri.ie/void#keiale> ,
                                                                    <http://vocab.deri.ie/void#Michael%20Hausenblas> ;
                                 <http://purl.org/dc/terms/modified> "2019-01-30"^^xsd:date ;
                                 <http://purl.org/dc/terms/provenance> :MODIFIED_TARGET ;
                                 rdfs:comment "One of the two datasets linked by the virtual link."^^xsd:string ;
                                 rdfs:label "Target"^^xsd:string .


#################################################################
#    Data properties
#################################################################

###  http://purl.org/query/voidext#resourceMapping
:resourceMapping rdf:type owl:DatatypeProperty ,
                          owl:FunctionalProperty ;
                 rdfs:domain :SimpleLinkSet ;
                 rdfs:range rdfs:Literal ;
                 <http://purl.org/dc/terms/description> """Example of a value assigned with this property is the following 
    \"?objectsTarget a <urn:Example>. BIND(IF(contains(?objectsTarget, \"Example:\" ), IRI(concat(\"http://example.org/uniprot:\",strafter(?objectsTarget,\"Example:\"))), ?objectsTargetConverted)
         as ?converted_object)
     FILTER(BOUND(?obj_converted))\". 
     This will convert strings that contains \"Example:\" into IRIs defined in http://example.org/ namespace."""^^xsd:string ;
                 rdfs:comment """The preprocessing of a resource (i.e. IRI or literal) in a source void:Dataset in order
to match another resource in the target void:Dataset. A resource is either the subject or the 
object of an RDF triple. The resource preprocessing (i.e. the resource mapping)
must be defined with the SPARQL language by mainly using SPARQL built-ins for assignments
(e.g. BIND), and expression and testing values (e.g. IF and FILTER). BIND is used to assign
the output of a function."""^^xsd:string ;
                 rdfs:label "resource mapped with"@en .


###  http://rdfs.org/ns/void#classes
<http://rdfs.org/ns/void#classes> rdf:type owl:DatatypeProperty ;
                                  rdfs:domain <http://rdfs.org/ns/void#Dataset> ;
                                  rdfs:range xsd:integer ;
                                  <http://purl.org/dc/terms/creator> <http://vocab.deri.ie/void#cygri> ,
                                                                     <http://vocab.deri.ie/void#junzha> ,
                                                                     <http://vocab.deri.ie/void#keiale> ,
                                                                     <http://vocab.deri.ie/void#Michael%20Hausenblas> ;
                                  rdfs:comment "The total number of distinct classes in a void:Dataset. In other words, the number of distinct resources occuring as objects of rdf:type triples in the dataset."^^xsd:string ;
                                  rdfs:isDefinedBy <http://vocab.deri.ie/void> ;
                                  rdfs:label "classes"^^xsd:string .


###  http://rdfs.org/ns/void#distinctObjects
<http://rdfs.org/ns/void#distinctObjects> rdf:type owl:DatatypeProperty ;
                                          rdfs:domain <http://rdfs.org/ns/void#Dataset> ;
                                          rdfs:range xsd:integer ;
                                          <http://purl.org/dc/terms/creator> <http://vocab.deri.ie/void#cygri> ,
                                                                             <http://vocab.deri.ie/void#junzha> ,
                                                                             <http://vocab.deri.ie/void#keiale> ,
                                                                             <http://vocab.deri.ie/void#Michael%20Hausenblas> ;
                                          rdfs:comment "The total number of distinct objects in a void:Dataset. In other words, the number of distinct resources that occur in the object position of triples in the dataset. Literals are included in this count."^^xsd:string ;
                                          rdfs:isDefinedBy <http://vocab.deri.ie/void> ;
                                          rdfs:label "distinct objects"^^xsd:string .


###  http://rdfs.org/ns/void#distinctSubjects
<http://rdfs.org/ns/void#distinctSubjects> rdf:type owl:DatatypeProperty ;
                                           rdfs:domain <http://rdfs.org/ns/void#Dataset> ;
                                           rdfs:range xsd:integer ;
                                           <http://purl.org/dc/terms/creator> <http://vocab.deri.ie/void#cygri> ,
                                                                              <http://vocab.deri.ie/void#junzha> ,
                                                                              <http://vocab.deri.ie/void#keiale> ,
                                                                              <http://vocab.deri.ie/void#Michael%20Hausenblas> ;
                                           rdfs:comment "The total number of distinct subjects in a void:Dataset. In other words, the number of distinct resources that occur in the subject position of triples in the dataset."^^xsd:string ;
                                           rdfs:isDefinedBy <http://vocab.deri.ie/void> ;
                                           rdfs:label "distinct subjects"^^xsd:string .


###  http://rdfs.org/ns/void#documents
<http://rdfs.org/ns/void#documents> rdf:type owl:DatatypeProperty ;
                                    rdfs:domain <http://rdfs.org/ns/void#Dataset> ;
                                    rdfs:range xsd:integer ;
                                    <http://purl.org/dc/terms/creator> <http://vocab.deri.ie/void#cygri> ,
                                                                       <http://vocab.deri.ie/void#junzha> ,
                                                                       <http://vocab.deri.ie/void#keiale> ,
                                                                       <http://vocab.deri.ie/void#Michael%20Hausenblas> ;
                                    rdfs:comment "The total number of documents, for datasets that are published as a set of individual documents, such as RDF/XML documents or RDFa-annotated web pages. Non-RDF documents, such as web pages in HTML or images, are usually not included in this count. This property is intended for datasets where the total number of triples or entities is hard to determine. void:triples or void:entities should be preferred where practical."^^xsd:string ;
                                    rdfs:isDefinedBy <http://vocab.deri.ie/void> ;
                                    rdfs:label "number of documents"^^xsd:string .


###  http://rdfs.org/ns/void#entities
<http://rdfs.org/ns/void#entities> rdf:type owl:DatatypeProperty ;
                                   rdfs:domain <http://rdfs.org/ns/void#Dataset> ;
                                   rdfs:range xsd:integer ;
                                   <http://purl.org/dc/terms/creator> <http://vocab.deri.ie/void#cygri> ,
                                                                      <http://vocab.deri.ie/void#junzha> ,
                                                                      <http://vocab.deri.ie/void#keiale> ,
                                                                      <http://vocab.deri.ie/void#Michael%20Hausenblas> ;
                                   rdfs:comment "The total number of entities that are described in a void:Dataset."^^xsd:string ;
                                   rdfs:isDefinedBy <http://vocab.deri.ie/void> ;
                                   rdfs:label "number of entities"^^xsd:string .


###  http://rdfs.org/ns/void#properties
<http://rdfs.org/ns/void#properties> rdf:type owl:DatatypeProperty ;
                                     rdfs:domain <http://rdfs.org/ns/void#Dataset> ;
                                     rdfs:range xsd:integer ;
                                     <http://purl.org/dc/terms/creator> <http://vocab.deri.ie/void#cygri> ,
                                                                        <http://vocab.deri.ie/void#junzha> ,
                                                                        <http://vocab.deri.ie/void#keiale> ,
                                                                        <http://vocab.deri.ie/void#Michael%20Hausenblas> ;
                                     rdfs:comment "The total number of distinct properties in a void:Dataset. In other words, the number of distinct resources that occur in the predicate position of triples in the dataset."^^xsd:string ;
                                     rdfs:isDefinedBy <http://vocab.deri.ie/void> ;
                                     rdfs:label "number of properties"^^xsd:string .


###  http://rdfs.org/ns/void#triples
<http://rdfs.org/ns/void#triples> rdf:type owl:DatatypeProperty ;
                                  rdfs:domain <http://rdfs.org/ns/void#Dataset> ;
                                  rdfs:range xsd:integer ;
                                  <http://purl.org/dc/terms/creator> <http://vocab.deri.ie/void#cygri> ,
                                                                     <http://vocab.deri.ie/void#junzha> ,
                                                                     <http://vocab.deri.ie/void#keiale> ,
                                                                     <http://vocab.deri.ie/void#Michael%20Hausenblas> ;
                                  rdfs:comment "The total number of triples contained in a void:Dataset."^^xsd:string ;
                                  rdfs:isDefinedBy <http://vocab.deri.ie/void> ;
                                  rdfs:label "number of triples"^^xsd:string .


###  http://rdfs.org/ns/void#uriSpace
<http://rdfs.org/ns/void#uriSpace> rdf:type owl:DatatypeProperty ;
                                   rdfs:domain <http://rdfs.org/ns/void#Dataset> ;
                                   rdfs:range rdfs:Literal ;
                                   <http://purl.org/dc/terms/creator> <http://vocab.deri.ie/void#cygri> ,
                                                                      <http://vocab.deri.ie/void#junzha> ,
                                                                      <http://vocab.deri.ie/void#keiale> ,
                                                                      <http://vocab.deri.ie/void#Michael%20Hausenblas> ;
                                   rdfs:comment "A URI that is a common string prefix of all the entity URIs in a void:Dataset."^^xsd:string ;
                                   rdfs:isDefinedBy <http://vocab.deri.ie/void> ;
                                   rdfs:label "URI space"^^xsd:string .


#################################################################
#    Classes
#################################################################

###  http://purl.org/dc/terms/Agent
<http://purl.org/dc/terms/Agent> rdf:type owl:Class .


###  http://purl.org/dc/terms/ProvenanceStatement
<http://purl.org/dc/terms/ProvenanceStatement> rdf:type owl:Class ;
                                               rdfs:isDefinedBy <http://purl.org/dc/terms/ProvenanceStatement> ;
                                               rdfs:label "Provenance Statement"^^xsd:string .


###  http://purl.org/query/voidext#ComplexLinkSet
:ComplexLinkSet rdf:type owl:Class ;
                rdfs:subClassOf :VirtualLink ;
                rdfs:comment "It is a complex virtual link. A complex link set is composed of exactly two link sets xor two shared instance sets where xor is the exclusive or. For example, two link sets that intersects at some graph node (e.g. the object nodes of link predicates)."@en ;
                rdfs:label "Complex link set"@en .


###  http://purl.org/query/voidext#LinkSetIntersection
:LinkSetIntersection rdf:type owl:Class ;
                     rdfs:comment "The possible intersection types between the RDF graph nodes in different void:Dataset(s) (i.e. either the subject or the object node of a link predicate). The instances of this class are exclusively voidext:OBJECT_OBJECT, voidext:OBJECT_SUBJECT, and voidext:SUBJECT_SUBJECT."@en ;
                     rdfs:label "Linkset intersection"@en .


###  http://purl.org/query/voidext#SharedInstanceSet
:SharedInstanceSet rdf:type owl:Class ;
                   rdfs:subClassOf :SimpleLinkSet ;
                   rdfs:comment "A simple link set between shared instances that are usually of the same OWL/RDFS class and asserted in two different datasets."@en ;
                   rdfs:label "Shared instance set"@en .


###  http://purl.org/query/voidext#SimpleLinkSet
:SimpleLinkSet rdf:type owl:Class ;
               rdfs:subClassOf :VirtualLink ;
               rdfs:comment "A simple link set must contain in its definition, either exactly one link predicate (void:linkPredicate) or exactly one shared instance type (i.e. class). The instances of this class must be also instances of its subclasses (i.e. void:Linkset xor voidext:SharedInstanceSet - where xor is the exclusive or)."@en ;
               rdfs:label "Simple link set"@en .


###  http://purl.org/query/voidext#VirtualLink
:VirtualLink rdf:type owl:Class ;
             rdfs:subClassOf <http://rdfs.org/ns/void#Dataset> ;
             rdfs:comment "A virtual link is a connection between resources such as literals and instances with some commonality. Each of these resources is from a different RDF dataset. Semantic relaxation is also considered when defining common resources between datasets. For example, the datasets uses different prefix namespaces for similar instances in a given domain scope. A virtual link can be interpreted as an intersection data point between two datasets. In addition, a virtual link is not concretely stored. The link may be physically established during a federated query execution, for example. This class must only have instances of its subclasses."@en ;
             rdfs:label "Virtual link set"@en .


###  http://rdfs.org/ns/void#Dataset
<http://rdfs.org/ns/void#Dataset> rdf:type owl:Class ;
                                  <http://purl.org/dc/terms/creator> <http://vocab.deri.ie/void#cygri> ,
                                                                     <http://vocab.deri.ie/void#junzha> ,
                                                                     <http://vocab.deri.ie/void#keiale> ,
                                                                     <http://vocab.deri.ie/void#Michael%20Hausenblas> ;
                                  rdfs:comment "A set of RDF triples that are published, maintained or aggregated by a single provider."^^xsd:string ;
                                  rdfs:isDefinedBy <http://vocab.deri.ie/void> ;
                                  rdfs:label "dataset"^^xsd:string .


###  http://rdfs.org/ns/void#DatasetDescription
<http://rdfs.org/ns/void#DatasetDescription> rdf:type owl:Class ;
                                             rdfs:subClassOf <http://xmlns.com/foaf/0.1/Document> ;
                                             <http://purl.org/dc/terms/creator> <http://vocab.deri.ie/void#cygri> ,
                                                                                <http://vocab.deri.ie/void#junzha> ,
                                                                                <http://vocab.deri.ie/void#keiale> ,
                                                                                <http://vocab.deri.ie/void#Michael%20Hausenblas> ;
                                             rdfs:comment "A web resource whose foaf:primaryTopic or foaf:topics include void:Datasets."^^xsd:string ;
                                             rdfs:isDefinedBy <http://vocab.deri.ie/void> ;
                                             rdfs:label "dataset description"^^xsd:string .


###  http://rdfs.org/ns/void#Linkset
<http://rdfs.org/ns/void#Linkset> rdf:type owl:Class ;
                                  rdfs:subClassOf :SimpleLinkSet ;
                                  <http://purl.org/dc/terms/contributor> <http://purl.org/query/tarcisiomf> ;
                                  <http://purl.org/dc/terms/created> "2010-01-26"^^xsd:date ;
                                  <http://purl.org/dc/terms/creator> <http://vocab.deri.ie/void#cygri> ,
                                                                     <http://vocab.deri.ie/void#junzha> ,
                                                                     <http://vocab.deri.ie/void#keiale> ,
                                                                     <http://vocab.deri.ie/void#Michael%20Hausenblas> ;
                                  <http://purl.org/dc/terms/modified> "2019-01-30"^^xsd:date ;
                                  <http://purl.org/dc/terms/provenance> :MODIFIED_LINKSET ;
                                  rdfs:comment "A collection of simple virtual links between two RDF datasets (i.e. void:Dataset). This collection is defined with exactly one RDF link predicate."^^xsd:string ;
                                  rdfs:label "linkset"^^xsd:string .


###  http://rdfs.org/ns/void#TechnicalFeature
<http://rdfs.org/ns/void#TechnicalFeature> rdf:type owl:Class ;
                                           <http://purl.org/dc/terms/creator> <http://vocab.deri.ie/void#cygri> ,
                                                                              <http://vocab.deri.ie/void#junzha> ,
                                                                              <http://vocab.deri.ie/void#keiale> ,
                                                                              <http://vocab.deri.ie/void#Michael%20Hausenblas> ;
                                           rdfs:comment "A technical feature of a void:Dataset, such as a supported RDF serialization format."^^xsd:string ;
                                           rdfs:isDefinedBy <http://vocab.deri.ie/void> ;
                                           rdfs:label "technical feature"^^xsd:string .


###  http://www.w3.org/1999/02/22-rdf-syntax-ns#Property
rdf:Property rdf:type owl:Class .


###  http://www.w3.org/2000/01/rdf-schema#Class
rdfs:Class rdf:type owl:Class .


###  http://www.w3.org/2000/01/rdf-schema#Resource
rdfs:Resource rdf:type owl:Class .


###  http://www.w3.org/ns/adms#SemanticAsset
<http://www.w3.org/ns/adms#SemanticAsset> rdf:type owl:Class .


###  http://www.w3.org/ns/sparql-service-description#Dataset
<http://www.w3.org/ns/sparql-service-description#Dataset> rdf:type owl:Class ;
                                                          rdfs:subClassOf <http://rdfs.org/ns/void#Dataset> .


###  http://www.w3.org/ns/sparql-service-description#Graph
<http://www.w3.org/ns/sparql-service-description#Graph> rdf:type owl:Class ;
                                                        rdfs:subClassOf <http://rdfs.org/ns/void#Dataset> .


###  http://xmlns.com/foaf/0.1/Document
<http://xmlns.com/foaf/0.1/Document> rdf:type owl:Class .


###  http://xmlns.com/foaf/0.1/Person
<http://xmlns.com/foaf/0.1/Person> rdf:type owl:Class .


#################################################################
#    Individuals
#################################################################

###  http://purl.org/query/tarcisiomf
<http://purl.org/query/tarcisiomf> rdf:type owl:NamedIndividual ,
                                            <http://xmlns.com/foaf/0.1/Person> ;
                                   <http://xmlns.com/foaf/0.1/homepage> <https://www.researchgate.net/profile/Tarcisio_Mendes_De_Farias> ;
                                   <http://xmlns.com/foaf/0.1/mbox> <mailto:tarcisio.mendesdefarias@unil.ch> ;
                                   <http://xmlns.com/foaf/0.1/name> "Tarcisio Mendes de Farias"^^xsd:string .


###  http://purl.org/query/voidext
<http://purl.org/query/voidext> rdf:type owl:NamedIndividual ,
                                         <http://www.w3.org/ns/adms#SemanticAsset> .


###  http://purl.org/query/voidext#MODIFIED_LINKSET
:MODIFIED_LINKSET rdf:type owl:NamedIndividual ,
                           <http://purl.org/dc/terms/ProvenanceStatement> ;
                  <http://purl.org/dc/terms/creator> <http://purl.org/query/tarcisiomf> ;
                  <http://purl.org/dc/terms/description> "The void:Linkset class was modified in voidext schema to be a subclass of voidext:SimpleLinkSet (that is subclass of voidext:VirtualLink) instead of void:Dataset class from the original VoID vocabulary. In addition, the voidext:VirtualLink is a subclass of void:Dataset. The rdfs:comment assertion was also improved."^^xsd:string ;
                  <http://purl.org/dc/terms/issued> "2019-01-30"^^xsd:date ;
                  <http://purl.org/dc/terms/label> "modified void:Linkset class"^^xsd:string .


###  http://purl.org/query/voidext#MODIFIED_TARGET
:MODIFIED_TARGET rdf:type owl:NamedIndividual ,
                          <http://purl.org/dc/terms/ProvenanceStatement> ;
                 <http://purl.org/dc/terms/creator> <http://purl.org/query/tarcisiomf> ;
                 <http://purl.org/dc/terms/description> "The void:target, void:subjectsTarget and void:objectsTarget VoID property domains were modified in voidext schema to be a superclass of void:Linkset, namely voidext:VirtualLink instead of void:Linkset class from the original VoID vocabulary. Therefore, all instances of voidext:VirtualLink including void:Linkset can use this property. The rdfs:comment assertion was also improved."^^xsd:string ;
                 <http://purl.org/dc/terms/issued> "2019-01-30"^^xsd:date ;
                 <http://purl.org/dc/terms/label> "modified property domain"^^xsd:string .


###  http://purl.org/query/voidext#OBJECT_OBJECT
:OBJECT_OBJECT rdf:type owl:NamedIndividual ,
                        :LinkSetIntersection ;
               rdfs:comment "The intersection between two void:Dataset(s) (i.e. knowledge graphs) occurs at the object node in both datasets."@en ;
               rdfs:label "Object-object intersection"@en .


###  http://purl.org/query/voidext#SUBJECT_OBJECT
:SUBJECT_OBJECT rdf:type owl:NamedIndividual ,
                         :LinkSetIntersection ;
                rdfs:comment "The intersection between two void:Dataset(s) (i.e. knowledge graphs) occurs at the object node of one data set (graph) and the subject node of another data set (graph)."@en ;
                rdfs:label "Subject-object intersection"@en .


###  http://purl.org/query/voidext#SUBJECT_SUBJECT
:SUBJECT_SUBJECT rdf:type owl:NamedIndividual ,
                          :LinkSetIntersection ;
                 rdfs:comment "The intersection between two void:Dataset(s) (i.e. knowledge graphs) occurs at the subject node in both datasets."@en ;
                 rdfs:label "Subject-subject intersection"@en .


###  http://vocab.deri.ie/void#LiDRC
<http://vocab.deri.ie/void#LiDRC> rdf:type owl:NamedIndividual ,
                                           <http://purl.org/dc/terms/Agent> ;
                                  <http://xmlns.com/foaf/0.1/homepage> <http://linkeddata.deri.ie/> ;
                                  <http://xmlns.com/foaf/0.1/member> <http://vocab.deri.ie/void#Michael%20Hausenblas> ;
                                  <http://xmlns.com/foaf/0.1/name> "LiDRC"^^xsd:string .


###  http://vocab.deri.ie/void#Talis
<http://vocab.deri.ie/void#Talis> rdf:type owl:NamedIndividual ,
                                           <http://purl.org/dc/terms/Agent> ;
                                  <http://xmlns.com/foaf/0.1/homepage> <http://www.talis.com/> ;
                                  <http://xmlns.com/foaf/0.1/member> <http://vocab.deri.ie/void#keiale> ;
                                  <http://xmlns.com/foaf/0.1/name> "Talis"^^xsd:string .


###  http://vocab.deri.ie/void#cygri
<http://vocab.deri.ie/void#cygri> rdf:type owl:NamedIndividual ,
                                           <http://xmlns.com/foaf/0.1/Person> ;
                                  <http://xmlns.com/foaf/0.1/homepage> <http://richard.cyganiak.de/> ;
                                  <http://xmlns.com/foaf/0.1/mbox> <mailto:richard.cyganiak@deri.org> ;
                                  <http://xmlns.com/foaf/0.1/name> "Richard Cyganiak"^^xsd:string .


###  http://vocab.deri.ie/void#junzha
<http://vocab.deri.ie/void#junzha> rdf:type owl:NamedIndividual ,
                                            <http://xmlns.com/foaf/0.1/Person> ;
                                   <http://xmlns.com/foaf/0.1/homepage> <http://users.ox.ac.uk/~zool0770/> ;
                                   <http://xmlns.com/foaf/0.1/mbox> <mailto:jun.zhao@zoo.ox.ac.uk> ;
                                   <http://xmlns.com/foaf/0.1/name> "Jun Zhao"^^xsd:string .


###  http://vocab.deri.ie/void#keiale
<http://vocab.deri.ie/void#keiale> rdf:type owl:NamedIndividual ,
                                            <http://xmlns.com/foaf/0.1/Person> ;
                                   <http://xmlns.com/foaf/0.1/homepage> <http://kwijibo.talis.com/> ;
                                   <http://xmlns.com/foaf/0.1/mbox> <mailto:Keith.Alexander@talis.com> ;
                                   <http://xmlns.com/foaf/0.1/name> "Keith Alexander"^^xsd:string .


###  http://vocab.deri.ie/void#Department%20of%20Zoology%2C%20University%20of%20Oxford
<http://vocab.deri.ie/void#Department%20of%20Zoology%2C%20University%20of%20Oxford> rdf:type owl:NamedIndividual ,
                                                                                             <http://purl.org/dc/terms/Agent> ;
                                                                                    <http://xmlns.com/foaf/0.1/homepage> <http://www.zoo.ox.ac.uk/> ;
                                                                                    <http://xmlns.com/foaf/0.1/member> <http://vocab.deri.ie/void#junzha> ;
                                                                                    <http://xmlns.com/foaf/0.1/name> "Department of Zoology, University of Oxford"^^xsd:string .


###  http://vocab.deri.ie/void#Digital%20Enterprise%20Research%20Institute%2C%20NUI%20Galway
<http://vocab.deri.ie/void#Digital%20Enterprise%20Research%20Institute%2C%20NUI%20Galway> rdf:type owl:NamedIndividual ,
                                                                                                   <http://purl.org/dc/terms/Agent> ;
                                                                                          <http://xmlns.com/foaf/0.1/homepage> <http://www.deri.ie/> ;
                                                                                          <http://xmlns.com/foaf/0.1/member> <http://vocab.deri.ie/void#cygri> ;
                                                                                          <http://xmlns.com/foaf/0.1/name> "Digital Enterprise Research Institute, NUI Galway"^^xsd:string .


###  http://vocab.deri.ie/void#Michael%20Hausenblas
<http://vocab.deri.ie/void#Michael%20Hausenblas> rdf:type owl:NamedIndividual ,
                                                          <http://xmlns.com/foaf/0.1/Person> ;
                                                 <http://xmlns.com/foaf/0.1/homepage> <http://sw-app.org/about.html> ;
                                                 <http://xmlns.com/foaf/0.1/mbox> <mailto:michael.hausenblas@deri.org> ;
                                                 <http://xmlns.com/foaf/0.1/name> "Michael Hausenblas"^^xsd:string .


###  Generated by the OWL API (version 5.1.0) https://github.com/owlcs/owlapi/
